Add reveal_at_least, a more clever form of reveal (#1167)
Depth determines which indices get expanded, but all references to the
same index get expanded if they appear in the output.

This is because Joel's latest examples require a rewriting pass that
needs either uneven revealing or the ability to check expression
equality modulo the dag in the middle of rewriting.
https://github.com/mit-plv/fiat-crypto/pull/1134#issuecomment-1075320548
Roughly the issue is that if we want to turn `a + 4 * a` into `5 * a`,
we need to reveal enough structure to see `4 * a`, but we need to see
that the two instances of `a` are the same (e.g., if `a` is an ExprRef
pointing to `b|c`, and we reveal uniformly, then we need to recognize
`b|c + 4 * a`)

src/Assembly/Symbolic.v
@@ -24,6 +24,7 @@ Require Import Crypto.Util.ListUtil.Filter.
 Require Import Crypto.Util.ListUtil.PermutationCompat. Import ListUtil.PermutationCompat.Coq.Sorting.Permutation.
 Require Import Crypto.Util.NUtil.Sorting.
 Require Import Crypto.Util.NUtil.Testbit.
+Require Import Crypto.Util.MSetN.
 Require Import Crypto.Util.ListUtil.PermutationCompat.
 Require Import Crypto.Util.Bool.LeCompat.
 Require Import Crypto.Util.Tactics.DestructHead.
@@ -238,6 +239,54 @@ Section WithDag.
   Definition reveal_node n '(op, args) :=
     ExprApp (op, List.map (reveal n) args).
 
+  (** given a set of indices, get the set of indices of their arguments *)
+  Definition reveal_gather_deps_args (ls : NSet.t) : NSet.t
+    := fold_right
+         (fun i so_far => match List.nth_error dag (N.to_nat i) with
+                          | None => so_far
+                          | Some (_op, args) => fold_right NSet.add so_far args
+                          end)
+         NSet.empty
+         (NSet.elements ls).
+
+  (** given a set of seen indices and a set of newly-revealed indices,
+  we want to merge the new indices into what's been seen and recurse
+  on the new indices *)
+  Definition reveal_gather_deps_step reveal_gather_deps (so_far : NSet.t) (new_idxs : NSet.t) : NSet.t
+    := let new_idxs := NSet.diff new_idxs so_far in
+       if NSet.is_empty new_idxs
+       then so_far
+       else reveal_gather_deps (NSet.union so_far new_idxs) (reveal_gather_deps_args new_idxs).
+
+  Fixpoint reveal_gather_deps_list (n : nat) (so_far : NSet.t) (new_idxs : NSet.t) : NSet.t
+    := match n with
+       | O => NSet.union so_far new_idxs
+       | S n => reveal_gather_deps_step (reveal_gather_deps_list n) so_far new_idxs
+       end.
+
+  Definition reveal_gather_deps (n : nat) (i : idx) : NSet.t
+    := reveal_gather_deps_list n NSet.empty (NSet.singleton i).
+
+  Definition reveal_step_from_deps reveal (deps : NSet.t) (i : idx) : expr
+    := if NSet.mem i deps
+       then match List.nth_error dag (N.to_nat i) with
+            | None => (* undefined *) ExprRef i
+            | Some (op, args) => ExprApp (op, List.map reveal args)
+            end
+       else ExprRef i.
+  Fixpoint reveal_from_deps_fueled (fuel : nat) (deps : NSet.t) (i : idx) :=
+    match fuel with
+    | O => ExprRef i
+    | S fuel => reveal_step_from_deps (reveal_from_deps_fueled fuel deps) deps i
+    end.
+  (** depth determines which indices get expanded, but all references
+  to the same index get expanded if they appear in the output *)
+  Definition reveal_at_least n (i : idx) : expr
+    := reveal_from_deps_fueled (S (List.length dag)) (reveal_gather_deps n i) i.
+
+  Definition reveal_node_at_least n '(op, args) :=
+    ExprApp (op, List.map (reveal_at_least n) args).
+
   Local Unset Elimination Schemes.
   Inductive eval : expr -> Z -> Prop :=
   | ERef i op args args' n
@@ -315,6 +364,35 @@ Section WithDag.
     eapply (proj1 (Forall2_map_l _ _ _)) in H0; eapply Forall2_map_l.
     eapply Forall2_weaken; try eassumption; []; cbv beta; intros.
     eapply eval_reveal; eauto.
+  Qed.
+
+  Lemma eval_reveal_from_deps_fueled deps : forall n i, forall v, eval (ExprRef i) v ->
+    forall e, reveal_from_deps_fueled n deps i = e -> eval e v.
+  Proof using Type.
+    induction n; cbn [reveal_from_deps_fueled]; cbv [reveal_step_from_deps]; intros; subst; eauto; [].
+    break_innermost_match_step; eauto; [].
+    inversion H; subst; clear H.
+    rewrite H1; econstructor; try eassumption; [].
+    eapply (proj1 (Forall2_map_l _ _ _)) in H2.
+    clear dependent i; clear dependent v.
+    induction H2; cbn; eauto.
+  Qed.
+
+  Lemma eval_reveal_at_least : forall n i, forall v, eval (ExprRef i) v ->
+    forall e, reveal_at_least n i = e -> eval e v.
+  Proof using Type.
+    cbv [reveal_at_least].
+    intros; eapply eval_reveal_from_deps_fueled; eassumption.
+  Qed.
+
+  Lemma eval_node_reveal_node_at_least : forall n v, eval_node n v ->
+    forall f e, reveal_node_at_least f n = e -> eval e v.
+  Proof using Type.
+    cbv [reveal_node]; inversion 1; intros; subst.
+    econstructor; eauto.
+    eapply (proj1 (Forall2_map_l _ _ _)) in H0; eapply Forall2_map_l.
+    eapply Forall2_weaken; try eassumption; []; cbv beta; intros.
+    eapply eval_reveal_at_least; eauto.
   Qed.
 End WithDag.
 
@@ -1950,10 +2028,10 @@ Qed.
 End Rewrite.
 
 Definition simplify (dag : dag) (e : node idx) :=
-  Rewrite.expr (reveal_node dag 3 e).
+  Rewrite.expr (reveal_node_at_least dag 3 e).
 
 Lemma eval_simplify G d n v : eval_node G d n v -> eval G d (simplify d n) v.
-Proof using Type. eauto using Rewrite.eval_expr, eval_node_reveal_node. Qed.
+Proof using Type. eauto using Rewrite.eval_expr, eval_node_reveal_node_at_least. Qed.
 
 Definition reg_state := Tuple.tuple (option idx) 16.
 Definition flag_state := Tuple.tuple (option idx) 6.
